Rewrite Match, haltConf, alternative While_Rels

TM/Combinators/Match.v
@@ -56,188 +56,318 @@ Section Match.
   Definition MATCH := (Match; Match_p).
   
 
+  (** Lift configurations of [M1] to configurations of [Match] *)
   Definition lift_confL (c : mconfig sig (states M1) n) : mconfig sig (states Match) n :=
     mk_mconfig (inl (cstate c)) (ctapes c).
 
+
+  (** Lift configuration of [M2] to configurations of [Match] *)
   Definition lift_confR (f : F) (c : mconfig sig (states (Mf f) ) n) : mconfig sig (states Match) n :=
     mk_mconfig (inr (existT (fun f0 : F => states (Mf f0)) f (cstate c))) (ctapes c).
-  (* Arguments lift_confR f c : clear implicits. *)
 
-  Lemma step_seq_liftL c0 :
-    halt (cstate c0) = false -> step (lift_confL c0) = lift_confL (step c0).
+  (** Lifted Steps of [M1] are compatible with steps in [M1], for non-halting states *)
+  Lemma step_comp_liftL (c : mconfig sig (states M1) n) :
+    halt (cstate c) = false -> lift_confL (step c) = step (lift_confL c).
   Proof.
-    destruct c0. unfold lift_confL, step. cbn. intros. destruct * eqn:_. now inv H1.
+    destruct c; cbn. unfold lift_confL, step. cbn. intros H. rewrite H.
+    destruct (trans _) eqn:E. cbn. reflexivity.
   Qed.
 
-  Lemma step_seq_liftR f (c0 : mconfig sig (states (Mf f)) n) :
-    step (lift_confR c0) = lift_confR (step c0).
+  (** Lifted steps of case-machines [Mf f] are compatible with steps in [Mf f] *)
+  Lemma step_comp_liftR f (c : mconfig sig (states (Mf f)) n) :
+    lift_confR (step c) = step (lift_confR c).
   Proof.
-    destruct c0. unfold lift_confR, step. cbn. destruct * eqn:_. now inv H0.
+    destruct c. unfold lift_confR, step. cbn.
+    destruct (trans _) eqn:E. cbn. reflexivity.
   Qed.
 
+  (** Lifted halting states of [M1] *)
   Definition halt_liftL (c : mconfig sig (states (Match)) n) :=
     match cstate c with
-    | inl s => halt (m := M1) s
-    | inr s => let (f, s) := s in halt (m := Mf f) s
+    | inl q => halt (m := M1) q
+    | inr q => halt (m := Mf (projT1 q)) (projT2 q)
     end.
 
-  Lemma Match_merge (k1 k2 : nat)
+
+  (** Non-halting states of [M1] are non-halting states of [Match] *)
+  Lemma halt_conf_liftL (c : mconfig sig (states Match) n) :
+    halt_liftL c = false -> halt (cstate c) = false.
+  Proof.
+    intros H. cbn. unfold Match_halt.
+    destruct c as [q t]; cbn.
+    destruct q; cbn in *; auto.
+  Qed.
+
+  (** The "nop" transition jumps from a halting configuration of [M1] to the initial configuration of the corresponding case-machine. *)
+  Lemma step_nop_transition (c : mconfig sig (states M1) n) :
+    haltConf c = true ->
+    step (lift_confL c) = lift_confR (initc (Mf (p1 (cstate c))) (ctapes c)).
+  Proof.
+    intros Halt.
+    unfold lift_confL, lift_confR. cbn. unfold haltConf in Halt.
+    unfold step at 1; cbn.
+    rewrite Halt. f_equal.
+    apply tape_move_null_action.
+  Qed.
+
+  (** The starting configuration of [Match] corresponds to the starting configuration of [M1]. *)
+  Lemma lift_initc t :
+    initc Match t = lift_confL (initc M1 t).
+  Proof. reflexivity. Qed.
+
+  (** This lemma is needed for the termination part. Suppose [M1] terminates in [c1].  The case machine [Mf f] starts with the tapes of [c1] and terminates in a configuration [c2]. Then, if we start [Match] with the same tapes as [M1], [Match] terminates in the lifted configuration of [c2]. *)
+  Lemma Match_merge t (k1 k2 : nat)
         (c1 : mconfig sig (states M1) n)
-        (c2 : mconfig sig (states (projT1 (pMf (p1 (cstate c1))))) n)
-        t:
+        (c2 : mconfig sig (states (Mf (p1 (cstate c1)))) n) :
     loopM k1 (initc M1 t) = Some c1 ->
     loopM k2 (initc (Mf (p1 (cstate c1))) (ctapes c1)) = Some c2 ->
     loopM (k1 + (1 + k2)) (initc Match t) = Some (lift_confR c2).
   Proof.
-    intros H H1.
-    unfold loopM.
-    eapply (loop_merge (p := halt_liftL) (a2 := lift_confL c1)).
-    - intros ? H3. cbn. unfold halt_liftL in H3. now destruct cstate as [ q | (f&q)].
-    - unfold loopM in H. cbn.
-      eapply loop_lift with (lift := lift_confL) (hlift := halt_liftL) in H; eauto.
-      + intuition. rewrite step_seq_liftL; eauto.
-    - change (loop (1 + k2) (step (M:=Match)) (fun c : mconfig sig (states Match) n => halt (cstate c)) (lift_confL c1)) with (loop k2 (step (M:=Match)) (fun c : mconfig sig (states Match) n => halt (cstate c)) (step (lift_confL c1))).
-      pose (M2 := (Mf (p1 (cstate c1)))).
-      eapply loop_lift with (lift := @lift_confR (p1 (cstate c1))) (hlift := (fun x => halt (m := Match) (cstate x))) in H1;eauto.
-      + cutrewrite  (step (lift_confL c1) = (lift_confR (initc M2 (ctapes c1)))); eauto.
-        destruct c1. unfold lift_confL, lift_confR. unfold step.
-        cbn -[null_action tape_move_multi]. cutrewrite (halt cstate = true). f_equal.
-        eapply tape_move_null_action. eapply loop_fulfills_p in H.
-        cbn in H; destruct (halt cstate); auto.
-      + intuition. now rewrite step_seq_liftR.
+    intros HLoop1 HLoop2. unfold loopM in *.
+    apply loop_merge with (p := halt_liftL) (a2 := lift_confL c1).
+    - apply halt_conf_liftL.
+    - rewrite lift_initc.
+      apply loop_lift with (h := haltConf (M := M1)) (f := step (M := M1)).
+      + unfold haltConf. intros. cbn. reflexivity.
+      + apply step_comp_liftL.
+      + apply HLoop1.
+    - (* execute one step *)
+      change (loop (1 + k2) (step (M:=Match)) (haltConf (M:=Match)) (lift_confL c1))
+        with (loop k2 (step (M:=Match)) (haltConf (M:=Match)) (step (lift_confL c1))).
+      eapply loop_lift with (lift := lift_confR (f := p1 (cstate c1))) (g := step (M := Match)) (hlift := haltConf (M := Match)) in HLoop2.
+      + rewrite <- HLoop2. f_equal. apply step_nop_transition. apply (loop_fulfills_p HLoop1).
+      + intros. cbn. reflexivity.
+      + intros. apply step_comp_liftR.
   Qed.
 
-  Definition unlift_1 : mconfig sig (FinType (EqType (states M1 + { f : F & TM.states (Mf f) }))) n -> option (mconfig sig (states M1) n).
+
+  (** The unlift functions map the configuration/state of [Match] to the corresponding states of either [M1] or some [Mf f]. *)
+  Definition unlift_confL : mconfig sig (states Match) n -> option (mconfig sig (states M1) n) :=
+    fun c =>
+      match (cstate c) with
+      | inl q => Some (mk_mconfig q (ctapes c))
+      | inr _ => None
+      end.
+
+  Definition unlift_confR (f : F) : mconfig sig (states Match) n -> option (mconfig sig (states (Mf f)) n).
   Proof.
-    intros m. destruct m. destruct cstate. left. econstructor. exact e. exact ctapes. right.
+    cbn in *.
+    refine (fun c =>
+              match (cstate c) with
+              | inl _ => None
+              | inr q => _
+              end).
+    destruct q as [y q]. decide (y = f) as [e | _].
+    - refine (Some (mk_mconfig _ (ctapes c))).
+      rewrite <- e. apply q.
+    - apply None.
   Defined.
 
-  Definition unlift_2 f : mconfig sig (FinType (EqType (states M1 + { f : F & TM.states (Mf f) }))) n -> option (mconfig sig (states (Mf f)) n).
-  Proof.
-    intros m. destruct m. destruct cstate.
-    - right.
-    - destruct s as [f' e].
-      decide (f = f').
-      + left. econstructor. symmetry in e0. rewrite <- e0. exact e. exact ctapes.
-      + right.
-  Defined.
 
-  Lemma unlift_2_step f (a : mconfig sig (states Match) n)( a' : mconfig sig (states (Mf f)) n) :
-    unlift_2 f a = Some a' -> halt (cstate a') = false -> unlift_2 f (step a) = Some (step a').
+  (** The lift and unlift functions are retracts. *)
+  Lemma retract_L (c : mconfig sig (states Match) n) (c' : mconfig sig (states M1) n) :
+    unlift_confL c = Some c' -> c = lift_confL c'.
   Proof.
-    destruct a. unfold unlift_2, step, trans. cbn. intros.
-    destruct cstate eqn:E; inv H. cbn in *. destruct s. decide (f = x); subst; inv H2. cbn in *.
-    destruct * eqn:E. rewrite <- Eqdep_dec.eq_rect_eq_dec;[ |apply eqType_dec].
-    inv H. inv H1. inv H2.
-
-    assert (((existT (fun f0 : F => states (Mf f0)) x0 e2), t1) =
-            ((existT (fun f : F => states (Mf f)) x0 e0), t0)). congruence.
-    assert (t1 = t0). congruence.
-    assert (((existT (fun f0 : F => states (Mf f0)) x0 e2)) =
-            ((existT (fun f : F => states (Mf f)) x0 e0))). congruence.
-    eapply eq_sigT_iff_eq_dep in H2. eapply Eqdep_dec.eq_dep_eq_dec in H2; eauto.
-    subst.
-    revert H7 H5. clear. destruct (Mf x0).
-    intros. unfold TM.trans in *. rewrite H7 in H5. congruence.
-    intros. eapply eqType_dec.
+    destruct c as [q t]. unfold unlift_confL, lift_confL. cbn. intros H.
+    destruct q as [ q | ?]; inv H. cbn. reflexivity.
   Qed.
 
-  Lemma unlift_1_step (a : mconfig sig (states Match) n)
-        ( a' : mconfig sig (states M1) n) : unlift_1 a = Some a' -> halt (cstate a') = false -> unlift_1 (step a) = Some (step a').
+  Lemma retract_L' (f : F) (c : mconfig sig (states M1) n) :
+    unlift_confL (lift_confL c) = Some c.
+  Proof. destruct c as [q t]. unfold unlift_confL, lift_confL. cbn. reflexivity. Qed.
+  
+
+  Lemma retract_R (f : F) (c : mconfig sig (states Match) n) (c' : mconfig sig (states (Mf f)) n) :
+    unlift_confR f c = Some c' -> c = lift_confR c'.
   Proof.
-    destruct a. unfold unlift_1, step, trans. cbn. intros.
-    destruct cstate eqn:E; inv H. cbn in *. rewrite H0. unfold trans.
-    destruct M1. cbn in *. destruct trans. reflexivity.
+    destruct c as [q t]. unfold unlift_confR, lift_confR. cbn. intros H.
+    destruct q as [ q | [y q]]. inv H.
+    decide (y = f) as [ -> | ?]; inv H.
+    cbn. reflexivity.
   Qed.
 
-  Lemma Match_split i res t:
-    loopM i (initc Match t) = Some res ->
-    (exists i1 x1 i2 x2,  loopM i1 (initc M1 t) = Some x1 /\
-                     loopM i2 (initc (Mf (p1 (cstate x1))) (ctapes x1)) = Some x2 /\ i = 1 + i1 + i2 /\ res = (lift_confR x2)).
+  Lemma retract_R' (f : F) (c : mconfig sig (states (Mf f)) n) :
+    unlift_confR f (lift_confR c) = Some c.
   Proof.
-    intros.
-    unfold loopM in H.
-    eapply loop_split in H.
-    destruct H as (i1 & x1 & i2 & H1 & H2 & Hi).
-
-    eapply loop_unlift with (unlift := unlift_1)
-                            (f := step (M := M1))
-                            (p := fun c => halt (m := M1) (cstate c))
-      in H1 as (x' & Hx' & Hu).
-    exists i1, x'.
-    - unfold loopM at 1. rewrite Hx'.
-      destruct x1. unfold unlift_1 in Hu. cbn in Hu. destruct cstate; inv Hu.
-      destruct i2; try now inv H2. cbn -[halt] in H2. unfold halt at 1 in H2. cbn -[halt] in H2.
-      unfold step at 2 in H2. cbn -[halt] in H2.
-      assert (halt e = true). eapply loop_fulfills_p in Hx'. cbn in Hx'. cbn in Hx'. destruct (halt e); auto. rewrite H in H2.
-      remember (mk_mconfig (inr (existT (fun f : F => states (Mf f)) (p1 e) (start (Mf (p1 e)))))
-                           (Vector.map2 (tape_move_mono (sig:=sig)) ctapes
-                                        (Vector.const (None, N) n))) as x2.
-      pose (M2 := (Mf (p1 e))).
-      eapply loop_unlift with (unlift := unlift_2 (p1 e))
-                                (f := step (M := M2))
-                                (p := fun c => halt (m := M2) (cstate c))
-                                (p' := fun c => halt (m := Match) (cstate c))
-        in H2 as (x'' & Hx'' & Hu').
-      + exists i2. exists x''. intuition. eapply Hx''. omega. destruct x''. unfold lift_confR. cbn. destruct res. unfold unlift_2 in *. cbn in Hu'. destruct cstate0; inv Hu'. destruct s.  decide (p1 e = x); inv H1. reflexivity.
-      + intuition. now eapply unlift_2_step.
-      + intuition. cbn. unfold halt. destruct b. cbn in *.
-        destruct cstate. inv H0. inv H0. cbn. destruct s.  decide (p1 e = x); inv H3. reflexivity.
-      + subst. cbn. assert (T := tape_move_null_action ctapes). cbn in T. unfold tape_move_multi in T.
-        rewrite T. decide (p1 e = p1 e); try tauto.
-        unfold initc. f_equal. f_equal.
-        (* assert (p e = eqType_X ( type (@states sig n (Mf (p e))))). *)
-        rewrite <- Eqdep_dec.eq_rect_eq_dec;[ |apply eqType_dec].
-        reflexivity.
-    - intuition. now eapply unlift_1_step.
-    - intros. instantiate (1 := fun x => match cstate x with inl s => halt (m := M1) s | _ => true end).
-      cbn. unfold unlift_1 in H. destruct b, cstate. inv H. reflexivity. inv H.
-    - cbn. reflexivity.
-    - intros. cbn in *. destruct cstate. reflexivity. inv H0.
+    destruct c as [q t]. unfold unlift_confR, lift_confR. cbn. decide (f=f); try tauto.
+    f_equal. f_equal.
+    erewrite <- Eqdep_dec.eq_rect_eq_dec; auto. apply eqType_dec.
   Qed.
 
 
+  (** If the configuration [c] of [Match] corresponds to the non-halting configuration [c'] of [M1], then [Match] simulates the step a step from [c']. *)
+  Lemma unlift_confL_step (c : mconfig sig (states Match) n) (c' : mconfig sig (states M1) n) :
+    unlift_confL c = Some c' ->
+    haltConf c' = false ->
+    unlift_confL (step c) = Some (step c').
+  Proof.
+    intros HUnlift HHalt. unfold haltConf in HHalt.
+    destruct c as [q t]. cbn in *.
+    unfold unlift_confL in *. cbn in *.
+    destruct q; inv HUnlift.
+    unfold step; cbn in *. rewrite HHalt.
+    now destruct trans.
+  Qed.
+  
+  (** If the configuration [c] of [Match] corresponds to the non-halting configuration [c'] of [Mf f], then [Match] simulates the step a step from [c']. *)
+  Lemma unlift_confR_step f (c : mconfig sig (states Match) n) (c' : mconfig sig (states (Mf f)) n) :
+    unlift_confR f c = Some c' ->
+    haltConf c' = false ->
+    unlift_confR f (step c) = Some (step c').
+  Proof.
+    intros HUnlift HHalt.
+    destruct c as [q t]. cbn in *.
+    unfold step. cbn [cstate ctapes].
+    unfold unlift_confR in *. cbn [cstate ctapes] in HUnlift.
+    destruct q as [q | [y q]]. inv HUnlift.
+    decide (y=f) as [ -> | _].
+    - inv HUnlift. cbn in *.
+      destruct (trans (q, current_chars t)) as [nextq acts] eqn:E. cbn.
+      decide (f=f); try tauto. f_equal. f_equal.
+      erewrite <- Eqdep_dec.eq_rect_eq_dec; auto. apply eqType_dec.
+    - inv HUnlift.
+  Qed.
+
+
+  (** Is the configuration [c] of [Match] a halting state of [M1] or no state of [M1] at all? *)
+  Definition halt_unliftL : mconfig sig (states Match) n -> bool :=
+    fun c =>
+      match unlift_confL c with
+      | Some c' => haltConf c'
+      | None => default (* this is no configuration of [M1] *)
+      end.
+
+
+  Lemma halt_comp_unliftL (c : mconfig sig (states Match) n) :
+    halt_unliftL c = false ->
+    haltConf c = false.
+  Proof.
+    destruct c as [q t]. cbn. unfold halt_unliftL, unlift_confL. cbn.
+    intros H. destruct q as [q | ?]; cbn in *; auto.
+  Qed.
+
+  (** If [c] is a state of [Match] that corresponds to a state [c'] of [M1], then the values of the halting functions are compatible. *)
+  Lemma halt_sim_unliftL (c : mconfig sig (states Match) n) (c' : mconfig sig (states M1) n) :
+    unlift_confL c = Some c' ->
+    haltConf c' = halt_unliftL c.
+  Proof. intros -> % retract_L. cbn. now destruct c'. Qed.
+
+
+  (* XXX: Has it to be true or false? *)
+  Arguments default : simpl never.
+
+  Definition halt_unliftR (f : F) : mconfig sig (states Match) n -> bool :=
+    fun c =>
+      match unlift_confR f c with
+      | Some c' => haltConf c'
+      | None => default (* this is no configuration of [Mf f] *)
+      end.
+
+  Lemma halt_sim_unliftR (f : F) (c : mconfig sig (states Match) n) (c' : mconfig sig (states (Mf f)) n) :
+    unlift_confR f c = Some c' ->
+    haltConf c' = halt_unliftR f c.
+  Proof.
+    intros -> % retract_R.
+    unfold halt_unliftR, unlift_confR. cbn.
+    decide (f=f); try tauto.
+    destruct c'; cbn. f_equal. f_equal.
+    erewrite <- Eqdep_dec.eq_rect_eq_dec; auto. apply eqType_dec.
+  Qed.
+    
+
+  (** The [Match] machine must take the "nop" action if it is in a final state of [M1]. *)
+  Lemma step_nop_split (k2 : nat) (c2 : mconfig sig (states M1) n) (outc : mconfig sig (states Match) n) :
+    haltConf c2 = true ->
+    loop k2 (step (M:=Match)) (haltConf (M:=Match)) (lift_confL c2) = Some outc ->
+    exists k2' c2',
+      k2 = S k2' /\
+      loopM (M := Mf (p1 (cstate c2))) k2' (initc _ (ctapes c2)) = Some c2' /\
+      outc = lift_confR c2'.
+  Proof.
+    unfold loopM. intros HHalt HLoop2. unfold haltConf in HHalt.
+    destruct k2 as [ | k2'].
+    - inv HLoop2.
+    - exists k2'. cbn in HLoop2.
+      replace (step (lift_confL c2)) with (lift_confR (initc (Mf (p1 (cstate c2))) (ctapes c2))) in HLoop2; cycle 1.
+      { cbv [step]. cbn -[tape_move_multi]. rewrite HHalt. rewrite tape_move_null_action. reflexivity. }
+      apply loop_unlift with (unlift := @unlift_confR (p1 (cstate c2)))
+                              (a := initc (Mf (p1 (cstate c2))) (ctapes c2))
+                              (f := step (M := Mf (p1 (cstate c2))))
+                              (p := haltConf (M := Mf (p1 (cstate c2)))) in HLoop2
+        as (c2'&HLoop2&HLoop2').
+      + apply retract_R in HLoop2' as ->.  exists c2'. repeat split; auto.
+      + intros. now apply unlift_confR_step.
+      + intros ? ? -> % retract_R. cbn. now destruct a.
+      + apply retract_R'.
+  Qed.
+
+
+  Lemma Match_split i t (outc : mconfig sig (states Match) n) :
+    loopM i (initc Match t) = Some outc ->
+    exists k1 (c1 : mconfig sig (states M1) n) k2 (c2 : mconfig sig (states (Mf (p1 (cstate c1)))) n),
+      loopM k1 (initc M1 t) = Some c1 /\
+      loopM k2 (initc (Mf (p1 (cstate c1))) (ctapes c1)) = Some c2 /\
+      outc = lift_confR c2.
+  Proof.
+    unfold loopM. intros H.
+    apply loop_split with (p := halt_unliftL) in H as (k1&c1&k2&HLoop1&HLoop2&->).
+    - eapply loop_unlift with (unlift := unlift_confL) (a := initc M1 t) (f := step (M := M1)) (p := haltConf (M := M1)) in HLoop1
+        as (c1'&HLoop1&HLoop1').
+      + apply retract_L in HLoop1' as ->.
+        move HLoop2 at bottom.
+        apply step_nop_split in HLoop2 as (k2'&c2'&->&HLoop2&->). 2: exact (loop_fulfills_p HLoop1).
+        exists k1, c1', k2', c2'. auto.
+      + intros. now apply unlift_confL_step.
+      + intros. now apply halt_sim_unliftL.
+      + reflexivity.
+    - apply halt_comp_unliftL.
+  Qed.
+
+
+  
+  (** Correctness *)
   Lemma Match_Realise (R1 : Rel _ (F * _)) (R2 : F -> Rel _ (F' * _)) :
     pM1 ⊨ R1 ->
     (forall f : F, pMf f ⊨ R2 f) -> MATCH ⊨ (⋃_f (R1 |_ f) ∘ R2 f).
   Proof.
-    intros HR1 HR2 t1 i1 oenc2 eq.
-    hnf.
-    apply Match_split in eq as (?&?&?&?&Eq1&Eq2&->&->).
-    unfold Realise in HR1.
-    eapply HR1 in Eq1.
-    eapply HR2 in Eq2.
-    eexists _, _. split. eapply Eq1. eapply Eq2.
+    intros HRel1 HRel2. hnf in HRel1.
+    hnf. intros t i outc HLoop.
+    apply Match_split in HLoop as (k1&c1&k2&c2&HLoop1&HLoop2&->). cbn.
+    exists (p1 (cstate c1)), (ctapes c1). split.
+    - apply (HRel1 _ _ _ HLoop1).
+    - apply (HRel2 _ _ _ _ HLoop2).
   Qed.
 
 
-  Lemma Match_RealiseIn
-        (R1 : Rel _ (F * _)) (R2 : F -> Rel _ (F' * _)) k1 k2:
+  (** Runtime *)
+  Lemma Match_TerminatesIn (R1 : Rel _ (F * _)) T1 T2 :
+    pM1 ⊨ R1 -> M1 ↓ T1 -> (forall f : F, Mf f ↓(T2 f)) ->
+    projT1 MATCH ↓ (fun tin i => exists i1 i2, T1 tin i1 /\ 1 + i1 + i2 <= i /\ forall tout yout, R1 tin (yout, tout) -> T2 yout tout i2).
+  Proof.
+    unfold MATCH. intros HRel1 HTerm1 HTerm2. hnf in HRel1, HTerm1.
+    hnf. intros t i (i1&i2&HT1&Hk&H).
+    specialize HTerm1 with (1 := HT1) as (c1&HLoop1).
+    specialize HRel1 with (1 := HLoop1).
+    specialize H with (1 := HRel1).
+    specialize (HTerm2 _ _ _ H) as (c2&HLoop2).
+    pose proof Match_merge HLoop1 HLoop2 as HLoop.
+    exists (lift_confR c2). eapply loop_ge. 2: apply HLoop. omega.
+  Qed.
+
+
+  (** Correct + constant runtime *)
+  Lemma Match_RealiseIn (R1 : Rel _ (F * _)) (R2 : F -> Rel _ (F' * _)) k1 k2:
     pM1 ⊨c(k1) R1 ->
     (forall f : F, pMf f ⊨c(k2) R2 f) ->
     MATCH ⊨c(1 + k1 + k2) (⋃_f (R1 |_ f) ∘ R2 f).
   Proof.
-    intros HR1 HR2 t.
-    specialize (HR1 t) as (c' & ? & ?).
-    specialize (HR2 (projT2 pM1 (cstate c')) (ctapes c')) as (outc & ? & ?).
-    exists (lift_confR outc). split.
-    -  unfold loopM. eapply loop_ge with (k1:=k1+(1+k2)). omega.
-       now eapply Match_merge.
-    - cbn. firstorder.      
+    intros (H1&H2) % Realise_total H3. apply Realise_total. split.
+    - eapply Match_Realise; eauto. intros ?. eapply Realise_total; eauto.
+    - eapply TerminatesIn_monotone.
+      + apply Match_TerminatesIn; eauto. intros ?. eapply Realise_total; eauto.
+      + firstorder.
   Qed.
 
-  Lemma Match_TerminatesIn (R1 : Rel _ (F * _)) T1 T2 :
-    pM1 ⊨ R1 -> M1 ↓ T1 -> (forall f : F, Mf f ↓(T2 f)) ->
-    Match ↓ (fun tin i => exists i1 i2, T1 tin i1 /\ 1 + i1 + i2 <= i /\ forall tout yout, R1 tin (yout, tout) -> T2 yout tout i2).
-  Proof.
-    intros Real1 Term1 Term2.
-    hnf. intros tin i. intros (i1&i2&T3&Hi&T4).
-    hnf in Term1. specialize (Term1 _ _ T3) as (outc1&Hloop1).
-    hnf in Real1. specialize (Real1 _ _ _ Hloop1).
-    specialize (T4 _ _ Real1).
-    specialize (Term2 (p1 (cstate outc1))). hnf in Term2. specialize (Term2 _ _ T4) as (outc2&Hloop2).
-    exists (lift_confR outc2). eapply loop_ge with (k1:=i1+(1+i2)). omega. eapply Match_merge; eauto.
-  Qed.
 
 End Match.
 (* Arguments MATCH {n} {sig} {F} pM1 {_} pMf : clear implicits. *)
